miniML refactoring
Refactoring miniML to try to minimize the number of proof cases.

examples/miniML/miniMLProofsScript.sml
@@ -1,7 +1,7 @@
-open bossLib Theory Parse res_quanTheory Defn Tactic boolLib
-open finite_mapTheory listTheory pairTheory pred_setTheory
-open set_relationTheory sortingTheory stringTheory wordsTheory
-open MiniMLTheory
+open bossLib Theory Parse res_quanTheory Defn Tactic boolLib;
+open finite_mapTheory listTheory pairTheory pred_setTheory;
+open set_relationTheory sortingTheory stringTheory wordsTheory;
+open MiniMLTheory;
 
 open lcsymtacs;
 
@@ -54,14 +54,18 @@ val _ = save_thm ("type_subst_ind", type_subst_ind);
 
 (* ------------------------------------------------------------------------- *)
 
-(* Prove that never gets stuck if there is still work to do (i.e., it must
- * detect all type errors *)
+(* Prove that the small step semantics never gets stuck if there is still work
+ * to do (i.e., it must detect all type errors *)
 
 val untyped_safety_thm = Q.store_thm ("untyped_safety_thm",
 `∀envC env ds st. 
-  (d_step (envC, env, ds, st) = Stuck) = (ds = []) ∧ (st = NONE)`,
-rw [d_step_def, e_step_def, continue_def, push_def, return_def] >>
-every_case_tac);
+  (d_step (envC, env, ds, st) = Dstuck) = (ds = []) ∧ (st = NONE)`,
+rw [d_step_def, e_step_def, continue_def, push_def, return_def, 
+    type_error_def] >>
+every_case_tac >>
+fs [LET_THM, do_app_def] >>
+every_case_tac >>
+fs []);
 
 (* --------------------------- Type soundness ------------------------------- *)
 
@@ -95,7 +99,7 @@ val type_lookup_lem = Q.prove (
   ⇒
   (∃v'. lookup s env = SOME v')`,
 induct_on `env` >>
-rw [Once type_e_cases, lookup_def, bind_def] >>
+rw [Once type_v_cases, lookup_def, bind_def] >>
 fs [lookup_def] >|
 [CCONTR_TAC >>
      fs [] >>
@@ -119,7 +123,15 @@ val type_es_length_lem = Q.prove (
 `∀tenvC tenv es ts.
   type_es tenvC tenv es ts ⇒ (LENGTH es = LENGTH ts)`,
 induct_on `es` >>
-rw [Once type_e_cases] >>
+rw [Once type_v_cases] >>
+rw [] >>
+metis_tac []);
+
+val type_vs_length_lem = Q.prove (
+`∀tenvC vs ts.
+  type_vs tenvC vs ts ⇒ (LENGTH vs = LENGTH ts)`,
+induct_on `vs` >>
+rw [Once type_v_cases] >>
 rw [] >>
 metis_tac []);
 
@@ -143,11 +155,11 @@ cases_on `ts` >>
 fs [] >>
 EQ_TAC >>
 rw [] >|
-[pop_assum (ASSUME_TAC o SIMP_RULE (srw_ss ()) [Once type_e_cases]) >>
+[pop_assum (ASSUME_TAC o SIMP_RULE (srw_ss ()) [Once type_v_cases]) >>
      fs [],
- pop_assum (ASSUME_TAC o SIMP_RULE (srw_ss ()) [Once type_e_cases]) >>
+ pop_assum (ASSUME_TAC o SIMP_RULE (srw_ss ()) [Once type_v_cases]) >>
      fs [],
- metis_tac [type_e_rules], 
+ metis_tac [type_v_rules], 
  imp_res_tac type_es_length_lem >>
      fs [],
  imp_res_tac type_es_length_lem >>
@@ -160,15 +172,55 @@ rw [] >|
      fs [],
  imp_res_tac type_es_length_lem >>
      fs [],
- pop_assum (ASSUME_TAC o SIMP_RULE (srw_ss ()) [Once type_e_cases]) >>
+ pop_assum (ASSUME_TAC o SIMP_RULE (srw_ss ()) [Once type_v_cases]) >>
      fs [] >>
      metis_tac [],
- pop_assum (ASSUME_TAC o SIMP_RULE (srw_ss ()) [Once type_e_cases]) >>
+ pop_assum (ASSUME_TAC o SIMP_RULE (srw_ss ()) [Once type_v_cases]) >>
      fs [] >>
-     metis_tac [type_e_rules],
- rw [Once type_e_cases] >>
-     pop_assum (ASSUME_TAC o SIMP_RULE (srw_ss ()) [Once type_e_cases]) >>
+     metis_tac [type_v_rules],
+ rw [Once type_v_cases] >>
+     pop_assum (ASSUME_TAC o SIMP_RULE (srw_ss ()) [Once type_v_cases]) >>
      fs []]);
+
+(* Typing lists of expressions from the end *)
+val type_vs_end_lem = Q.prove (
+`∀tenvC vs ts v t.
+  type_vs tenvC (vs++[v]) (ts++[t]) =
+  type_v tenvC v t ∧
+  type_vs tenvC vs ts`,
+induct_on `vs` >>
+rw [] >>
+cases_on `ts` >>
+fs [] >>
+EQ_TAC >>
+rw [] >|
+[pop_assum (ASSUME_TAC o SIMP_RULE (srw_ss ()) [Once type_v_cases]) >>
+     fs [],
+ pop_assum (ASSUME_TAC o SIMP_RULE (srw_ss ()) [Once type_v_cases]) >>
+     fs [],
+ metis_tac [type_v_rules], 
+ imp_res_tac type_vs_length_lem >>
+     fs [],
+ imp_res_tac type_vs_length_lem >>
+     fs [],
+ imp_res_tac type_vs_length_lem >>
+     fs [],
+ imp_res_tac type_vs_length_lem >>
+     fs [],
+ imp_res_tac type_vs_length_lem >>
+     fs [],
+ imp_res_tac type_vs_length_lem >>
+     fs [],
+ pop_assum (ASSUME_TAC o SIMP_RULE (srw_ss ()) [Once type_v_cases]) >>
+     fs [] >>
+     metis_tac [],
+ pop_assum (ASSUME_TAC o SIMP_RULE (srw_ss ()) [Once type_v_cases]) >>
+     fs [] >>
+     metis_tac [type_v_rules],
+ rw [Once type_v_cases] >>
+     pop_assum (ASSUME_TAC o SIMP_RULE (srw_ss ()) [Once type_v_cases]) >>
+     fs []]);
+
 
 (* Recursive functions have function type *)
 val type_funs_Tfn = Q.prove (
@@ -180,7 +232,7 @@ val type_funs_Tfn = Q.prove (
 induct_on `funs` >>
 rw [] >>
 qpat_assum `type_funs tenvC tenv funspat tenv'` 
-      (ASSUME_TAC o SIMP_RULE (srw_ss()) [Once type_e_cases]) >>
+      (ASSUME_TAC o SIMP_RULE (srw_ss()) [Once type_v_cases]) >>
 rw [] >>
 fs [lookup_def, emp_def, bind_def] >>
 cases_on `fn = n` >>
@@ -189,33 +241,33 @@ metis_tac []);
 
 (* Classifying values of basic types *)
 val canonical_values_thm = Q.prove (
-`∀tenvC tenv v t1 t2.
-  (type_e tenvC tenv (Val v) Tnum ⇒ (∃n. v = Lit (Num n))) ∧
-  (type_e tenvC tenv (Val v) Tbool ⇒ (∃n. v = Lit (Bool n))) ∧
-  (type_e tenvC tenv (Val v) (Tfn t1 t2) ⇒ 
+`∀tenvC v t1 t2.
+  (type_v tenvC v Tnum ⇒ (∃n. v = Lit (Num n))) ∧
+  (type_v tenvC v Tbool ⇒ (∃n. v = Lit (Bool n))) ∧
+  (type_v tenvC v (Tfn t1 t2) ⇒ 
     (∃env n e. v = Closure env n e) ∨
     (∃env funs n. v = Recclosure env funs n))`,
 rw [] >>
-fs [Once type_e_cases] >>
+fs [Once type_v_cases] >>
 rw [] >>
 metis_tac [type_funs_Tfn, t_distinct]);
 
 (* Well-typed pattern matches either match or not, but don't raise type errors
 * *)
 val pmatch_type_progress = Q.prove (
-`(∀envC p v env t tenv tenv' tenv''.
+`(∀envC p v env t tenv tenv'.
   consistent_con_env envC tenvC ∧
   consistent_con_env2 envC tenvC ∧
   type_p tenvC tenv p t tenv' ∧
-  type_e tenvC tenv'' (Val v) t
+  type_v tenvC v t
   ⇒
   (pmatch envC p v env = No_match) ∨
   (∃env'. pmatch envC p v env = Match env')) ∧
- (∀envC ps vs env ts tenv tenv' tenv''.
+ (∀envC ps vs env ts tenv tenv'.
   consistent_con_env envC tenvC ∧
   consistent_con_env2 envC tenvC ∧
   type_ps tenvC tenv ps ts tenv' ∧
-  type_es tenvC tenv'' (MAP Val vs) ts
+  type_vs tenvC vs ts
   ⇒
   (pmatch_list envC ps vs env = No_match) ∨
   (∃env'. pmatch_list envC ps vs env = Match env'))`,
@@ -223,59 +275,59 @@ HO_MATCH_MP_TAC pmatch_ind >>
 rw [] >>
 rw [pmatch_def] >>
 fs [lit_same_type_def] >|
-[fs [Once type_e_cases, Once type_p_cases, lit_same_type_def] >>
+[fs [Once type_v_cases, Once type_p_cases, lit_same_type_def] >>
      rw [] >>
      fs [],
- fs [Once (hd (CONJUNCTS type_e_cases)), 
+ fs [Once (hd (CONJUNCTS type_v_cases)), 
      Once (hd (CONJUNCTS type_p_cases))] >>
      rw [] >>
      fs [] >>
      imp_res_tac consistent_con_env_lem >>
      rw [] >>
-     metis_tac [type_ps_length_lem, type_es_length_lem, LENGTH_MAP],
- fs [Once type_p_cases, Once type_e_cases, consistent_con_env2_def] >>
+     metis_tac [type_ps_length_lem, type_vs_length_lem, LENGTH_MAP],
+ fs [Once type_p_cases, Once type_v_cases, consistent_con_env2_def] >>
      imp_res_tac consistent_con_env_lem >>
      rw [] >>
      res_tac >>
      fs [] >>
      rw [] >>
-     metis_tac [type_ps_length_lem, type_es_length_lem, LENGTH_MAP],
- fs [Once type_e_cases, Once type_p_cases, lit_same_type_def] >>
+     metis_tac [type_ps_length_lem, type_vs_length_lem, LENGTH_MAP],
+ fs [Once type_v_cases, Once type_p_cases, lit_same_type_def] >>
      rw [] >>
      fs [],
- fs [Once type_e_cases, Once type_p_cases, lit_same_type_def] >>
+ fs [Once type_v_cases, Once type_p_cases, lit_same_type_def] >>
      rw [] >>
      fs [],
- fs [Once type_e_cases, Once type_p_cases, lit_same_type_def] >>
+ fs [Once type_v_cases, Once type_p_cases, lit_same_type_def] >>
      rw [] >>
      fs [] >>
      metis_tac [type_funs_Tfn, t_distinct],
- fs [Once type_e_cases, Once type_p_cases, lit_same_type_def] >>
+ fs [Once type_v_cases, Once type_p_cases, lit_same_type_def] >>
      rw [] >>
      fs [],
- fs [Once type_e_cases, Once type_p_cases, lit_same_type_def] >>
+ fs [Once type_v_cases, Once type_p_cases, lit_same_type_def] >>
      rw [] >>
      fs [],
-  fs [Once type_e_cases, Once type_p_cases, lit_same_type_def] >>
+  fs [Once type_v_cases, Once type_p_cases, lit_same_type_def] >>
      rw [] >>
      fs [] >>
      metis_tac [type_funs_Tfn, t_distinct],
  qpat_assum `type_ps tenvC tenv (p::ps) ts tenv'` 
          (ASSUME_TAC o SIMP_RULE (srw_ss()) [Once type_p_cases]) >>
-     qpat_assum `type_es tenvC tenv'' (e::es) ts` 
-         (ASSUME_TAC o SIMP_RULE (srw_ss()) [Once type_e_cases]) >>
+     qpat_assum `type_vs tenvC (v::vs) ts` 
+         (ASSUME_TAC o SIMP_RULE (srw_ss()) [Once type_v_cases]) >>
      fs [] >>
      rw [] >>
      res_tac >>
      fs [] >>
      metis_tac [],
  imp_res_tac type_ps_length_lem >>
-     imp_res_tac type_es_length_lem >>
+     imp_res_tac type_vs_length_lem >>
      fs [] >>
      cases_on `ts` >>
      fs [],
  imp_res_tac type_ps_length_lem >>
-     imp_res_tac type_es_length_lem >>
+     imp_res_tac type_vs_length_lem >>
      fs [] >>
      cases_on `ts` >>
      fs []]);
@@ -289,7 +341,7 @@ val type_funs_lookup = Q.prove (
   (∃t. lookup fn env' = SOME t)`,
 Induct_on `funs` >>
 rw [] >>
-pop_assum (ASSUME_TAC o SIMP_RULE (srw_ss()) [Once type_e_cases]) >>
+pop_assum (ASSUME_TAC o SIMP_RULE (srw_ss()) [Once type_v_cases]) >>
 fs [] >>
 fs [lookup_def, bind_def] >>
 rw [] >>
@@ -304,7 +356,7 @@ val type_funs_lookup2 = Q.prove (
   (∃n e. find_recfun fn funs = SOME (n,e))`,
 Induct_on `funs` >>
 rw [] >>
-pop_assum (ASSUME_TAC o SIMP_RULE (srw_ss()) [Once type_e_cases]) >>
+pop_assum (ASSUME_TAC o SIMP_RULE (srw_ss()) [Once type_v_cases]) >>
 fs [] >>
 fs [lookup_def, bind_def, emp_def] >>
 rw [Once find_recfun_def] >>
@@ -318,7 +370,7 @@ val type_funs_distinct = Q.prove (
   ALL_DISTINCT (MAP (λ(x,y,z). x) funs)`,
 induct_on `funs` >>
 rw [] >>
-pop_assum (ASSUME_TAC o SIMP_RULE (srw_ss()) [Once type_e_cases]) >>
+pop_assum (ASSUME_TAC o SIMP_RULE (srw_ss()) [Once type_v_cases]) >>
 fs [] >>
 rw [MEM_MAP] >|
 [cases_on `y` >>
@@ -330,6 +382,39 @@ rw [MEM_MAP] >|
      metis_tac [type_funs_lookup, optionTheory.NOT_SOME_NONE],
  metis_tac []]);
 
+val type_op_cases = Q.prove (
+`!op t1 t2 t3.
+  type_op op t1 t2 t3 =
+  ((∃op'. op = Opn op') ∧ (t1 = Tnum) ∧ (t2 = Tnum) ∧ (t3 = Tnum)) ∨
+  ((∃op'. op = Opb op') ∧ (t1 = Tnum) ∧ (t2 = Tnum) ∧ (t3 = Tbool)) ∨
+  ((op = Opapp) ∧ (t1 = Tfn t2 t3))`,
+rw [type_op_def] >>
+every_case_tac >>
+fs [] >>
+metis_tac []);
+
+val type_e_val = Q.prove (
+`!cenv tenv v t.
+  type_e cenv tenv (Val v) t = type_v cenv v t`,
+rw [Once type_v_cases]);
+
+val type_es_val = Q.prove (
+`!cenv tenv vs ts.
+  type_es cenv tenv (MAP Val vs) ts = type_vs cenv vs ts`,
+induct_on `vs` >>
+rw [] >>
+rw [Once (hd (tl (tl (tl (CONJUNCTS type_v_cases)))))] >>
+rw [Once (hd (tl (tl (CONJUNCTS type_v_cases))))] >>
+fs [] >>
+cases_on `ts` >>
+fs [] >>
+rw [type_e_val]);
+ 
+val final_state_def = Define `
+  (final_state (Val v) [] = T) ∧
+  (final_state (Raise err) [] = T) ∧
+  (final_state _ _ = F)`;
+
 (* A well-typed expression state is either a value with no continuation, or it
 * can step to another state, or it steps to a BindError. *)
 val exp_type_progress = Q.prove (
@@ -337,49 +422,45 @@ val exp_type_progress = Q.prove (
   consistent_con_env envC tenvC ∧
   consistent_con_env2 envC tenvC ∧
   type_state tenvC (envC, env, e, c) t ∧
-  (e_step (envC, env, e, c) ≠ BindError) ∧
-  (c ≠ [])
+  ¬(final_state e c)
   ⇒
-  (∃env' e' c'. e_step (envC, env, e, c) = State (envC, env', e', c'))`,
+  (∃env' e' c'. e_step (envC, env, e, c) = Estep (envC, env', e', c'))`,
 rw [] >>
 rw [e_step_def] >>
-fs [type_state_cases, push_def] >>
+fs [type_state_cases, push_def, return_def] >>
 cases_on `e` >>
 fs [] >>
 rw [] >>
-fs [] >|
+fs [final_state_def] >|
 [rw [continue_def] >>
      fs [Once type_ctxts_cases, type_ctxt_cases, return_def, push_def] >>
      rw [] >>
+     fs [final_state_def] >>
+     every_case_tac >>
+     fs [type_e_val] >>
+     fs [type_op_cases] >>
+     rw [] >>
      imp_res_tac canonical_values_thm >>
      fs [] >>
+     rw [] >>
+     fs [do_app_def, do_if_def, do_log_def] >>
+     every_case_tac >>
      fs [] >|
-     [imp_res_tac type_funs_lookup2 >>
+     [qpat_assum `type_v tenvC (Recclosure x1 x2 x3) tpat`
+                (ASSUME_TAC o SIMP_RULE (srw_ss()) [Once type_v_cases]) >>
+          fs [] >>
+          imp_res_tac type_funs_lookup2 >>
           fs [],
-      metis_tac [log_nchotomy],
-      metis_tac [log_nchotomy],
-      metis_tac [log_nchotomy],
-      metis_tac [log_nchotomy],
-      metis_tac [log_nchotomy],
-      metis_tac [log_nchotomy],
-      metis_tac [log_nchotomy],
-      cases_on `pes` >>
-            rw [] >-
-            fs [e_step_def, continue_def] >>
-            fs [] >>
-            cases_on `h` >>
-            fs [RES_FORALL] >>
-            rw [] >>
-            qpat_assum `∀x. (x = (q,r)) ∨ P x ⇒ Q x` 
-                     (MP_TAC o Q.SPEC `(q,r)`) >>
-                rw [] >>
-                `(pmatch envC q v env' = No_match) ∨
-                 (∃env. pmatch envC q v env' = Match env)` by 
-                            metis_tac [pmatch_type_progress] >>
-                rw [],
-      cases_on `es` >>
-          rw []],
- fs [Once type_e_cases] >>
+      fs [RES_FORALL] >>
+          rw [] >>
+          qpat_assum `∀x. (x = (q,r)) ∨ P x ⇒ Q x` 
+                   (MP_TAC o Q.SPEC `(q,r)`) >>
+              rw [] >>
+              `(pmatch envC q v env' = No_match) ∨
+               (∃env. pmatch envC q v env' = Match env)` by 
+                          metis_tac [pmatch_type_progress] >>
+              fs []],
+ fs [Once type_v_cases] >>
      rw [] >>
      fs [] >>
      imp_res_tac consistent_con_env_lem >>
@@ -388,7 +469,7 @@ fs [] >|
      fs [return_def] >>
      imp_res_tac type_es_length_lem >>
      fs [],
- fs [Once type_e_cases] >>
+ fs [Once type_v_cases] >>
      rw [] >>
      fs [lookup_def, bind_def] >>
      imp_res_tac type_lookup_lem >>
@@ -397,35 +478,8 @@ fs [] >|
      fs [] >>
      res_tac >>
      rw [],
- fs [Once type_e_cases] >>
+ fs [Once type_v_cases] >>
      metis_tac [type_funs_distinct]]);
-
-(* It doesn't matter what environment we use to type values, because they have
-* no free variables. *)
-val type_val_weaken_stengthen_lem = Q.prove (
-`(∀(tenvC : tenvC) env e t.
-  type_e tenvC env e t ⇒
-  (∃v. e = Val v) ⇒
-  ∀env'. type_e tenvC env' e t) ∧
- (∀(tenvC : tenvC) env es ts.
-  type_es tenvC env es ts ⇒ 
-  (∃vs. es = MAP Val vs) ⇒
-  (∀env'. type_es tenvC env' es ts)) ∧
- (∀(tenvC : tenvC) env tenv.
-  type_env tenvC env tenv ⇒ T) ∧
- (∀(tenvC : tenvC) env funs env'.
-  type_funs tenvC env funs env' ⇒ T)`,
-HO_MATCH_MP_TAC type_e_strongind >>
-rw [] >>
-rw [Once type_e_cases] >|
-[metis_tac [],
- metis_tac [],
- metis_tac [],
- all_tac,
- all_tac] >>
-cases_on `vs` >>
-fs [] >>
-metis_tac []);
 
 (* They value of a binding in the execution environment has the type given by
 * the type environment. *)
@@ -442,43 +496,42 @@ fs [lookup_def] >>
 rw [] >>
 cases_on `tenv` >>
 fs [] >-
-fs [Once type_e_cases, bind_def] >>
+fs [Once type_v_cases, bind_def] >>
 fs [lookup_def] >>
 cases_on `h` >>
 cases_on `h'` >>
 qpat_assum `type_env tenvC ((q,r)::env) ((q',r')::t)`
-         (ASSUME_TAC o SIMP_RULE (srw_ss ()) [Once type_e_cases]) >>
+         (ASSUME_TAC o SIMP_RULE (srw_ss ()) [Once type_v_cases]) >>
 fs [bind_def] >>
 rw [] >>
 fs [lookup_def] >>
 cases_on `q = s` >>
 fs [] >>
 rw [] >>
-metis_tac [type_val_weaken_stengthen_lem]);
+metis_tac [type_e_val]);
 
 (* A successful pattern match gives a binding environment with the type given by
 * the pattern type checker *)
 val pmatch_type_preservation = Q.prove (
 `(∀envC p v env env' (tenvC:tenvC) tenv.
   (pmatch envC p v env = Match env') ∧
-  (∃t. type_e tenvC tenv (Val v) t) ∧
+  (∃t. type_v tenvC v t) ∧
   type_env tenvC env tenv ⇒
   ∃tenv'. type_env tenvC env' tenv') ∧
  (∀envC ps vs env env' (tenvC:tenvC) tenv.
   (pmatch_list envC ps vs env = Match env') ∧
-  (∃ts. type_es tenvC tenv (MAP Val vs) ts) ∧
+  (∃ts. type_vs tenvC vs ts) ∧
   type_env tenvC env tenv ⇒
   ∃tenv'. type_env tenvC env' tenv')`,
 HO_MATCH_MP_TAC pmatch_ind >>
 rw [pmatch_def] >|
 [qexists_tac `(n,t) :: tenv` >>
-     rw [Once type_e_cases, bind_def] >>
-     metis_tac [type_val_weaken_stengthen_lem],
+     rw [Once type_v_cases, bind_def, type_e_val],
  metis_tac [],
  every_case_tac >>
-     fs [] >>
-     qpat_assum `type_e tenvC tenv epat t`
-             (ASSUME_TAC o SIMP_RULE (srw_ss()) [Once type_e_cases]) >>
+     fs [type_e_val] >>
+     qpat_assum `type_v tenvC vpat t`
+             (ASSUME_TAC o SIMP_RULE (srw_ss()) [Once type_v_cases]) >>
      fs [] >>
      metis_tac [],
  every_case_tac >>
@@ -486,11 +539,10 @@ rw [pmatch_def] >|
  metis_tac [],
  every_case_tac >>
      fs [] >>
-     qpat_assum `type_es tenvC tenv (Val v::es) ts`
-             (ASSUME_TAC o SIMP_RULE (srw_ss ()) [Once type_e_cases]) >>
+     qpat_assum `type_vs tenvC (v::vs) ts`
+             (ASSUME_TAC o SIMP_RULE (srw_ss ()) [Once type_v_cases]) >>
      fs [] >>
-     metis_tac [SIMP_RULE (srw_ss ()) [] 
-                          type_val_weaken_stengthen_lem]]);
+     metis_tac []]);
 
 val build_rec_env_help_lem = Q.prove (
 `∀funs env funs'.
@@ -518,15 +570,15 @@ Induct_on `env'` >>
 rw [merge_def] >>
 cases_on `tenv'`>>
 fs [] >>
-rw [Once type_e_cases] >|
+rw [Once type_v_cases] >|
 [qpat_assum `type_env tenvC [] (h::t)`
-         (ASSUME_TAC o SIMP_RULE (srw_ss()) [Once type_e_cases]) >>
+         (ASSUME_TAC o SIMP_RULE (srw_ss()) [Once type_v_cases]) >>
      fs [bind_def],
  qpat_assum `type_env tenvC (h::env') []`
-         (ASSUME_TAC o SIMP_RULE (srw_ss()) [Once type_e_cases]) >>
+         (ASSUME_TAC o SIMP_RULE (srw_ss()) [Once type_v_cases]) >>
      fs [bind_def],
  qpat_assum `type_env tenvC (h::env') (h'::t)`
-         (ASSUME_TAC o SIMP_RULE (srw_ss()) [Once type_e_cases]) >>
+         (ASSUME_TAC o SIMP_RULE (srw_ss()) [Once type_v_cases]) >>
      fs [bind_def, merge_def] >>
      rw []]);
 
@@ -540,7 +592,7 @@ val type_recfun_lookup = Q.prove (
 induct_on `funs` >>
 rw [Once find_recfun_def] >>
 qpat_assum `type_funs tenvC tenv (h::funs) tenv'` 
-            (ASSUME_TAC o SIMP_RULE (srw_ss ()) [Once type_e_cases]) >>
+            (ASSUME_TAC o SIMP_RULE (srw_ss ()) [Once type_v_cases]) >>
 rw [] >>
 fs [] >>
 cases_on `fn' = fn` >>
@@ -558,10 +610,11 @@ val type_recfun_env_help = Q.prove (
   type_env tenvC (MAP (λ(fn,n,e). (fn,Recclosure env funs' fn)) funs) tenv`,
 induct_on `funs` >>
 rw [] >>
-pop_assum (ASSUME_TAC o SIMP_RULE (srw_ss ()) [Once type_e_cases]) >>
+pop_assum (ASSUME_TAC o SIMP_RULE (srw_ss ()) [Once type_v_cases]) >>
 fs [emp_def] >>
-rw [bind_def, Once type_e_cases] >|
-[rw [Once type_e_cases] >>
+rw [bind_def, Once type_v_cases] >|
+[rw [type_e_val] >>
+     rw [Once type_v_cases] >>
      metis_tac [lookup_def, bind_def],
  metis_tac [optionTheory.NOT_SOME_NONE, lookup_def, bind_def]]);
 
@@ -573,12 +626,18 @@ val type_recfun_env = Q.prove (
   type_env tenvC (MAP (λ(fn,n,e). (fn,Recclosure env funs fn)) funs) tenv`,
 metis_tac [type_recfun_env_help]);
 
+val type_v_lit = Q.prove (
+`(!tenvC n t. type_v tenvC (Lit (Num n)) t = (t = Tnum)) ∧
+ (!tenvC b t. type_v tenvC (Lit (Bool b)) t = (t = Tbool))`,
+rw [Once type_v_cases] >>
+rw [Once type_v_cases]);
+
 (* If a step can be taken from a well-typed state, the resulting state has the
 * same type *)
 val exp_type_preservation = Q.prove (
 `∀(tenvC:tenvC) envC env e c t env' e' c'.
   type_state tenvC (envC, env, e, c) t ∧
-  (e_step (envC, env, e, c) = State (envC, env', e', c'))
+  (e_step (envC, env, e, c) = Estep (envC, env', e', c'))
   ⇒
   type_state tenvC (envC, env', e', c') t`,
 rw [type_state_cases] >>
@@ -586,155 +645,138 @@ fs [e_step_def] >>
 cases_on `e` >>
 fs [push_def] >>
 rw [] >|
-[fs [continue_def, push_def] >>
+[every_case_tac >>
+     fs [emp_def] >>
+     rw [] >>
+     qexists_tac `t` >>
+     qexists_tac `[]` >>
+     rw [] >>
+     rw [Once type_v_cases, Once type_ctxts_cases],
+ fs [continue_def, push_def] >>
      cases_on `c` >>
      fs [] >>
      cases_on `h` >>
      fs [] >>
      cases_on `q` >>
-     fs [] >|
-     [every_case_tac >>
-          fs [] >|
-          [fs [Once type_ctxts_cases, type_ctxt_cases] >>
-               rw [] >>
-               metis_tac [type_val_weaken_stengthen_lem],
-           qpat_assum `type_ctxts tenvC (cpat::t') t1 t`
-                      (ASSUME_TAC o 
-                       SIMP_RULE (srw_ss()) [Once type_ctxts_cases]) >> 
-               fs [type_ctxt_cases] >>
-               rw [Once type_ctxts_cases, type_ctxt_cases] >>
-               qpat_assum `type_e tenvC tenv epat tpat`
-                      (ASSUME_TAC o 
-                       SIMP_RULE (srw_ss()) [Once type_e_cases]) >> 
-               metis_tac []],
-      every_case_tac >>
-          fs [] >>
-          qpat_assum `type_ctxts tenvC ((Capp2 l s e (),r)::c') t1 t`
-            (ASSUME_TAC o SIMP_RULE (srw_ss()) [Once type_ctxts_cases]) >> 
-          fs [type_ctxt_cases] >>
-          qpat_assum `type_e tenvC tenv' (Val (Closure l s e)) (Tfn t1 t2)`
-              (ASSUME_TAC o SIMP_RULE (srw_ss()) [Once type_e_cases]) >> 
-          rw [] >>
-          metis_tac [type_e_rules, type_val_weaken_stengthen_lem, bind_def],
-      every_case_tac >>
-          fs [] >>
-          qpat_assum `type_ctxts tenvC ((Capp3 l l0 s (),r)::c') t1 t`
-            (ASSUME_TAC o SIMP_RULE (srw_ss()) [Once type_ctxts_cases]) >> 
-          fs [type_ctxt_cases] >>
-          rw [build_rec_env_lem] >>
-
-          imp_res_tac type_recfun_lookup >>
-          qexists_tac `t2` >>
-          qexists_tac `(bind q t1 (merge tenv''' tenv''))` >>
-          rw [] >>
-          rw [Once type_e_cases, bind_def] >-
-          metis_tac [type_val_weaken_stengthen_lem] >>
-          match_mp_tac type_env_merge_lem >>
-          rw [] >>
-          metis_tac [type_recfun_env],
-      every_case_tac >>
-          fs [return_def] >>
-          fs [] >>
-          rw [] >>
-          qpat_assum `type_ctxts tenvC cpat t1 t`
-            (ASSUME_TAC o SIMP_RULE (srw_ss()) [Once type_ctxts_cases]) >> 
-          fs [type_ctxt_cases] >>
-          rw [] >>
-          metis_tac [type_val_weaken_stengthen_lem],
-      every_case_tac >>
-          fs [] >>
-          rw [] >>
-          fs [Once type_ctxts_cases, type_ctxt_cases] >>
-          metis_tac [type_val_weaken_stengthen_lem],
-      every_case_tac >>
-          fs [return_def] >>
-          fs [] >>
-          rw [] >>
-          qpat_assum `type_ctxts tenvC cpat t1 t`
-            (ASSUME_TAC o SIMP_RULE (srw_ss()) [Once type_ctxts_cases]) >> 
-          fs [type_ctxt_cases] >> 
-          metis_tac [type_e_rules],
-      every_case_tac >>
-          fs [] >>
-          rw [] >>
-          qpat_assum `type_ctxts tenvC cpat t1 t`
-            (ASSUME_TAC o SIMP_RULE (srw_ss()) [Once type_ctxts_cases]) >> 
-          fs [type_ctxt_cases] >>
-          rw [] >>
+     fs [type_e_val] >>
+     every_case_tac >>
+     fs [return_def, type_error_def] >>
+     rw [] >>
+     pop_assum (ASSUME_TAC o 
+                SIMP_RULE (srw_ss()) [Once type_ctxts_cases]) >> 
+     fs [type_ctxt_cases] >>
+     rw [] >>
+     fs [type_e_val] >|
+     [rw [Once type_ctxts_cases, type_ctxt_cases, type_e_val] >>
           metis_tac [],
-      every_case_tac >>
-          fs [] >>
+      fs [do_app_def] >>
+          cases_on `o'` >>
+          fs [] >|
+          [every_case_tac >>
+               fs [] >>
+               rw [type_e_val] >>
+               fs [hd (CONJUNCTS type_v_cases)] >>
+               rw [] >>
+               fs [type_op_cases] >>
+               rw [] >>
+               metis_tac [],
+           every_case_tac >>
+               fs [] >>
+               rw [type_e_val] >>
+               fs [hd (CONJUNCTS type_v_cases)] >>
+               rw [] >>
+               fs [type_op_cases] >>
+               rw [] >>
+               metis_tac [],
+           every_case_tac >>
+               fs [] >>
+               rw [type_e_val] >|
+               [qpat_assum `type_v tenvC (Closure l s e) t1'`
+                     (ASSUME_TAC o SIMP_RULE (srw_ss()) [Once type_v_cases]) >> 
+                    fs [] >>
+                    rw [] >>
+                    fs [type_op_cases] >>
+                    rw [] >>
+                    qexists_tac `t2` >>
+                    qexists_tac `bind s t1 tenv''` >>
+                    rw [Once type_v_cases, type_e_val] >>
+                    metis_tac [],
+                qpat_assum `type_v tenvC (Recclosure l l0 s) t1'`
+                     (ASSUME_TAC o SIMP_RULE (srw_ss()) [Once type_v_cases]) >> 
+                    fs [] >>
+                    rw [] >>
+                    fs [type_op_cases] >>
+                    rw [] >>
+                    qexists_tac `t2` >>
+                    rw [build_rec_env_lem] >>
+                    imp_res_tac type_recfun_lookup >>
+                    qexists_tac `bind q t1 (merge tenv''' tenv'')` >>
+                    rw [bind_def, Once type_v_cases, type_e_val] >>
+                    metis_tac [type_env_merge_lem, type_recfun_env]]],
+      fs [do_log_def] >>
+           every_case_tac >>
+           fs [] >>
+           rw [type_e_val] >>
+           metis_tac [],
+      fs [do_if_def] >>
+           every_case_tac >>
+           fs [] >>
+           rw [type_e_val] >>
+           metis_tac [],
+      rw [Once (hd (tl (CONJUNCTS type_v_cases)))] >>
+          metis_tac [],
+      rw [Once type_ctxts_cases, type_ctxt_cases, type_e_val] >>
+          fs [RES_FORALL] >>
+          metis_tac [],
+      fs [RES_FORALL, FORALL_PROD] >>
           rw [] >>
-          qpat_assum `type_ctxts tenvC cpat t1 t`
-            (ASSUME_TAC o SIMP_RULE (srw_ss()) [Once type_ctxts_cases]) >> 
-          fs [type_ctxt_cases, RES_FORALL, FORALL_PROD] >>
-          rw [] >|
-          [rw [Once type_ctxts_cases, type_ctxt_cases,FORALL_PROD,RES_FORALL] >>
-               metis_tac [type_val_weaken_stengthen_lem],
-           metis_tac [type_val_weaken_stengthen_lem,
-                      pmatch_type_preservation]],
-      every_case_tac >>
-          fs [] >>
-          qpat_assum `type_ctxts tenvC cpat t1 t`
-            (ASSUME_TAC o SIMP_RULE (srw_ss()) [Once type_ctxts_cases]) >> 
-          fs [type_ctxt_cases] >>
-          rw [] >>
-          qexists_tac `t2` >>
+          metis_tac [pmatch_type_preservation],
+      qexists_tac `t2` >>
           qexists_tac `bind s t1 tenv'` >>
+          rw [Once type_v_cases, type_e_val] >>
+          metis_tac [],
+      rw [Once (hd (CONJUNCTS type_v_cases))] >>
+          imp_res_tac type_es_length_lem >>
+          fs [] >>
+          `ts2 = []` by 
+                  (cases_on `ts2` >>
+                   fs []) >>
+          rw [type_vs_end_lem] >>
+          fs [] >>
           rw [] >>
-          rw [Once type_e_cases, bind_def] >>
-          metis_tac [type_val_weaken_stengthen_lem],
-      every_case_tac >>
-          fs [return_def] >>                 
-          rw [] >|
-          [qpat_assum `type_ctxts tenvC cpat t1 t`
-            (ASSUME_TAC o SIMP_RULE (srw_ss()) [Once type_ctxts_cases]) >> 
-               fs [type_ctxt_cases] >>
-               qexists_tac `t2` >>
-               qexists_tac `tenv'` >>
-               rw [] >>
-               rw [Once type_e_cases] >>
-               imp_res_tac type_es_length_lem >>
-               fs [] >>
-               `ts2 = []` by 
-                       (cases_on `ts2` >>
-                        fs []) >>
-               rw [type_es_end_lem] >>
-               metis_tac [rich_listTheory.MAP_REVERSE, 
-                          type_val_weaken_stengthen_lem],
-           fs [type_ctxt_cases, Once type_ctxts_cases] >>
-               rw [] >>
-               qpat_assum `type_es tenvC tenv' (e'::t'') ts2`
-                     (ASSUME_TAC o SIMP_RULE (srw_ss()) [Once type_e_cases]) >> 
-               fs [] >>
-               rw [] >>
-               qexists_tac `t''''` >>
-               qexists_tac `tenv'` >>
-               rw [] >>
-               qexists_tac `tenv'` >>
-               qexists_tac `Tapp ts' tn` >>
-               rw [] >>
-               cases_on `ts2` >>
-               fs [] >>
-               rw [] >>
-               qexists_tac `ts1++[t''']` >>
-               qexists_tac `t'''''` >>
-               rw [] >>
-               metis_tac [type_es_end_lem, type_val_weaken_stengthen_lem]]],
+          metis_tac [type_es_val, rich_listTheory.MAP_REVERSE],
+      qpat_assum `type_es tenvC tenv' (e'::t'') ts2`
+                (ASSUME_TAC o SIMP_RULE (srw_ss()) [Once type_v_cases]) >> 
+          fs [] >>
+          rw [] >>
+          qexists_tac `t''''` >>
+          qexists_tac `tenv'` >>
+          rw [] >>
+          rw [type_ctxt_cases, Once type_ctxts_cases] >>
+          rw [] >>
+          qexists_tac `tenv'` >>
+          qexists_tac `Tapp ts' tn` >>
+          rw [] >>
+          cases_on `ts2` >>
+          fs [] >>
+          rw [] >>
+          qexists_tac `ts1++[t''']` >>
+          rw [] >> 
+          metis_tac [type_es_end_lem, type_es_val, type_e_val]],
  every_case_tac >>
-     fs [return_def] >>
+     fs [return_def, type_error_def] >>
      rw [] >>
      qpat_assum `type_e tenvC tenv (Con s epat) t1` 
-              (ASSUME_TAC o SIMP_RULE (srw_ss()) [Once type_e_cases]) >> 
+              (ASSUME_TAC o SIMP_RULE (srw_ss()) [Once type_v_cases]) >> 
      rw [] >>
      qpat_assum `type_es tenvC tenv epat ts` 
-              (ASSUME_TAC o SIMP_RULE (srw_ss()) [Once type_e_cases]) >> 
-     fs [] >|
+              (ASSUME_TAC o SIMP_RULE (srw_ss()) [Once type_v_cases]) >> 
+     fs [type_e_val] >|
      [qexists_tac `Tapp ts' tn` >>
           qexists_tac `tenv` >>
           rw [] >>
-          rw [Once type_e_cases] >>
-          rw [Once type_e_cases],
+          rw [Once type_v_cases] >>
+          rw [Once type_v_cases],
       rw [Once type_ctxts_cases, type_ctxt_cases] >>
           qexists_tac `t''`>>
           qexists_tac `tenv`>>
@@ -748,41 +790,43 @@ rw [] >|
           qexists_tac `[]` >>
           qexists_tac `t'''` >>
           rw [] >>
-          metis_tac [type_e_rules, APPEND]],
+          metis_tac [type_v_rules, APPEND]],
  every_case_tac >>
-     fs [] >>
+     fs [return_def, type_error_def] >>
      rw [] >>
      qexists_tac `t1` >>
      qexists_tac `tenv` >>
      rw [] >>
      qpat_assum `type_e tenvC tenv (Var s) t1` 
-              (ASSUME_TAC o SIMP_RULE (srw_ss()) [Once type_e_cases]) >> 
+              (ASSUME_TAC o SIMP_RULE (srw_ss()) [Once type_v_cases]) >> 
      metis_tac [type_lookup_lem2],
- fs [Once (hd (CONJUNCTS type_e_cases))] >>
+ fs [return_def] >>
+     rw [] >>
+     qpat_assum `type_e tenvC tenv (Fun s e'') t1` 
+              (ASSUME_TAC o SIMP_RULE (srw_ss()) [Once type_v_cases]) >> 
+     rw [type_e_val] >>
+     rw [Once (hd (CONJUNCTS type_v_cases))] >>
      metis_tac [],
- pop_assum (ASSUME_TAC o SIMP_RULE (srw_ss()) [Once type_e_cases]) >> 
+ pop_assum (ASSUME_TAC o SIMP_RULE (srw_ss()) [Once type_v_cases]) >> 
      rw [Once type_ctxts_cases, type_ctxt_cases] >>
      metis_tac [],
- pop_assum (ASSUME_TAC o SIMP_RULE (srw_ss()) [Once type_e_cases]) >> 
+ pop_assum (ASSUME_TAC o SIMP_RULE (srw_ss()) [Once type_v_cases]) >> 
      rw [Once type_ctxts_cases, type_ctxt_cases] >>
      metis_tac [],
- pop_assum (ASSUME_TAC o SIMP_RULE (srw_ss()) [Once type_e_cases]) >> 
+ pop_assum (ASSUME_TAC o SIMP_RULE (srw_ss()) [Once type_v_cases]) >> 
      rw [Once type_ctxts_cases, type_ctxt_cases] >>
      metis_tac [],
- pop_assum (ASSUME_TAC o SIMP_RULE (srw_ss()) [Once type_e_cases]) >> 
+ pop_assum (ASSUME_TAC o SIMP_RULE (srw_ss()) [Once type_v_cases]) >> 
      rw [Once type_ctxts_cases, type_ctxt_cases] >>
      metis_tac [],
- pop_assum (ASSUME_TAC o SIMP_RULE (srw_ss()) [Once type_e_cases]) >> 
-     rw [Once type_ctxts_cases, type_ctxt_cases] >>
-     metis_tac [],
- pop_assum (ASSUME_TAC o SIMP_RULE (srw_ss()) [Once type_e_cases]) >> 
+ pop_assum (ASSUME_TAC o SIMP_RULE (srw_ss()) [Once type_v_cases]) >> 
      rw [Once type_ctxts_cases, type_ctxt_cases] >>
      metis_tac [],
  every_case_tac >>
-     fs [] >>
+     fs [type_error_def] >>
      rw [] >>
      qpat_assum `type_e tenvC tenv epat t1`
-            (ASSUME_TAC o SIMP_RULE (srw_ss()) [Once type_e_cases]) >>
+            (ASSUME_TAC o SIMP_RULE (srw_ss()) [Once type_v_cases]) >>
      fs [] >>
      qexists_tac `t1` >>
      qexists_tac `merge tenv' tenv` >>
@@ -820,6 +864,7 @@ rw []);
 
 (* ------------------------ Big step/small step equivalence ----------------- *)
 
+(*
 val evaluate_ctxts_def = Q.prove (
 `∀ cenv v v' c env cs bv err.
   (evaluate_ctxts cenv [] v (Bvalue v') = (v = v')) ∧
@@ -869,6 +914,7 @@ CCONTR_TAC >>
 fs [] >>
 imp_res_tac big_exp_determ >>
 fs []);
+*)
 
 (*
 val exp_evaluation_preservation = Q.prove (
